AwsCryptographicMaterialProviders/runtimes/java/src/main/smithy-generated/software/amazon/cryptography/keystore/ToNative.java
@@ -13,17 +13,24 @@ import java.nio.ByteBuffer;
 import java.util.List;
 import java.util.Map;
 import software.amazon.cryptography.keystore.internaldafny.types.Error;
+import software.amazon.cryptography.keystore.internaldafny.types.Error_AlreadyExistsConditionFailed;
 import software.amazon.cryptography.keystore.internaldafny.types.Error_CollectionOfErrors;
 import software.amazon.cryptography.keystore.internaldafny.types.Error_KeyStorageException;
 import software.amazon.cryptography.keystore.internaldafny.types.Error_KeyStoreException;
+import software.amazon.cryptography.keystore.internaldafny.types.Error_MutationLockConditionFailed;
+import software.amazon.cryptography.keystore.internaldafny.types.Error_NoLongerExistsConditionFailed;
+import software.amazon.cryptography.keystore.internaldafny.types.Error_OldEncConditionFailed;
 import software.amazon.cryptography.keystore.internaldafny.types.Error_Opaque;
 import software.amazon.cryptography.keystore.internaldafny.types.Error_VersionRaceException;
 import software.amazon.cryptography.keystore.internaldafny.types.IKeyStoreClient;
 import software.amazon.cryptography.keystore.model.ActiveHierarchicalSymmetric;
 import software.amazon.cryptography.keystore.model.ActiveHierarchicalSymmetricBeacon;
+import software.amazon.cryptography.keystore.model.AlreadyExistsConditionFailed;
 import software.amazon.cryptography.keystore.model.AwsKms;
 import software.amazon.cryptography.keystore.model.BeaconKeyMaterials;
 import software.amazon.cryptography.keystore.model.BranchKeyMaterials;
+import software.amazon.cryptography.keystore.model.ClobberMutationLockInput;
+import software.amazon.cryptography.keystore.model.ClobberMutationLockOutput;
 import software.amazon.cryptography.keystore.model.CollectionOfErrors;
 import software.amazon.cryptography.keystore.model.CreateKeyInput;
 import software.amazon.cryptography.keystore.model.CreateKeyOutput;
@@ -49,6 +56,8 @@ import software.amazon.cryptography.keystore.model.GetItemsForInitializeMutation
 import software.amazon.cryptography.keystore.model.GetKeyStorageInfoInput;
 import software.amazon.cryptography.keystore.model.GetKeyStorageInfoOutput;
 import software.amazon.cryptography.keystore.model.GetKeyStoreInfoOutput;
+import software.amazon.cryptography.keystore.model.GetMutationLockInput;
+import software.amazon.cryptography.keystore.model.GetMutationLockOutput;
 import software.amazon.cryptography.keystore.model.HierarchicalKeyType;
 import software.amazon.cryptography.keystore.model.HierarchicalSymmetric;
 import software.amazon.cryptography.keystore.model.KMSConfiguration;
@@ -58,6 +67,9 @@ import software.amazon.cryptography.keystore.model.KeyStoreConfig;
 import software.amazon.cryptography.keystore.model.KeyStoreException;
 import software.amazon.cryptography.keystore.model.MRDiscovery;
 import software.amazon.cryptography.keystore.model.MutationLock;
+import software.amazon.cryptography.keystore.model.MutationLockConditionFailed;
+import software.amazon.cryptography.keystore.model.NoLongerExistsConditionFailed;
+import software.amazon.cryptography.keystore.model.OldEncConditionFailed;
 import software.amazon.cryptography.keystore.model.OpaqueError;
 import software.amazon.cryptography.keystore.model.QueryForVersionsInput;
 import software.amazon.cryptography.keystore.model.QueryForVersionsOutput;
@@ -98,6 +110,19 @@ public class ToNative {
     return nativeBuilder.build();
   }
 
+  public static AlreadyExistsConditionFailed Error(
+    Error_AlreadyExistsConditionFailed dafnyValue
+  ) {
+    AlreadyExistsConditionFailed.Builder nativeBuilder =
+      AlreadyExistsConditionFailed.builder();
+    nativeBuilder.message(
+      software.amazon.smithy.dafny.conversion.ToNative.Simple.String(
+        dafnyValue.dtor_message()
+      )
+    );
+    return nativeBuilder.build();
+  }
+
   public static KeyStorageException Error(
     Error_KeyStorageException dafnyValue
   ) {
@@ -120,6 +145,45 @@ public class ToNative {
     return nativeBuilder.build();
   }
 
+  public static MutationLockConditionFailed Error(
+    Error_MutationLockConditionFailed dafnyValue
+  ) {
+    MutationLockConditionFailed.Builder nativeBuilder =
+      MutationLockConditionFailed.builder();
+    nativeBuilder.message(
+      software.amazon.smithy.dafny.conversion.ToNative.Simple.String(
+        dafnyValue.dtor_message()
+      )
+    );
+    return nativeBuilder.build();
+  }
+
+  public static NoLongerExistsConditionFailed Error(
+    Error_NoLongerExistsConditionFailed dafnyValue
+  ) {
+    NoLongerExistsConditionFailed.Builder nativeBuilder =
+      NoLongerExistsConditionFailed.builder();
+    nativeBuilder.message(
+      software.amazon.smithy.dafny.conversion.ToNative.Simple.String(
+        dafnyValue.dtor_message()
+      )
+    );
+    return nativeBuilder.build();
+  }
+
+  public static OldEncConditionFailed Error(
+    Error_OldEncConditionFailed dafnyValue
+  ) {
+    OldEncConditionFailed.Builder nativeBuilder =
+      OldEncConditionFailed.builder();
+    nativeBuilder.message(
+      software.amazon.smithy.dafny.conversion.ToNative.Simple.String(
+        dafnyValue.dtor_message()
+      )
+    );
+    return nativeBuilder.build();
+  }
+
   public static VersionRaceException Error(
     Error_VersionRaceException dafnyValue
   ) {
@@ -133,11 +197,23 @@ public class ToNative {
   }
 
   public static RuntimeException Error(Error dafnyValue) {
+    if (dafnyValue.is_AlreadyExistsConditionFailed()) {
+      return ToNative.Error((Error_AlreadyExistsConditionFailed) dafnyValue);
+    }
     if (dafnyValue.is_KeyStorageException()) {
       return ToNative.Error((Error_KeyStorageException) dafnyValue);
     }
     if (dafnyValue.is_KeyStoreException()) {
       return ToNative.Error((Error_KeyStoreException) dafnyValue);
+    }
+    if (dafnyValue.is_MutationLockConditionFailed()) {
+      return ToNative.Error((Error_MutationLockConditionFailed) dafnyValue);
+    }
+    if (dafnyValue.is_NoLongerExistsConditionFailed()) {
+      return ToNative.Error((Error_NoLongerExistsConditionFailed) dafnyValue);
+    }
+    if (dafnyValue.is_OldEncConditionFailed()) {
+      return ToNative.Error((Error_OldEncConditionFailed) dafnyValue);
     }
     if (dafnyValue.is_VersionRaceException()) {
       return ToNative.Error((Error_VersionRaceException) dafnyValue);
@@ -252,6 +328,25 @@ public class ToNative {
         dafnyValue.dtor_branchKey()
       )
     );
+    return nativeBuilder.build();
+  }
+
+  public static ClobberMutationLockInput ClobberMutationLockInput(
+    software.amazon.cryptography.keystore.internaldafny.types.ClobberMutationLockInput dafnyValue
+  ) {
+    ClobberMutationLockInput.Builder nativeBuilder =
+      ClobberMutationLockInput.builder();
+    nativeBuilder.mutationLock(
+      ToNative.MutationLock(dafnyValue.dtor_mutationLock())
+    );
+    return nativeBuilder.build();
+  }
+
+  public static ClobberMutationLockOutput ClobberMutationLockOutput(
+    software.amazon.cryptography.keystore.internaldafny.types.ClobberMutationLockOutput dafnyValue
+  ) {
+    ClobberMutationLockOutput.Builder nativeBuilder =
+      ClobberMutationLockOutput.builder();
     return nativeBuilder.build();
   }
 
@@ -601,6 +696,31 @@ public class ToNative {
     nativeBuilder.kmsConfiguration(
       ToNative.KMSConfiguration(dafnyValue.dtor_kmsConfiguration())
     );
+    return nativeBuilder.build();
+  }
+
+  public static GetMutationLockInput GetMutationLockInput(
+    software.amazon.cryptography.keystore.internaldafny.types.GetMutationLockInput dafnyValue
+  ) {
+    GetMutationLockInput.Builder nativeBuilder = GetMutationLockInput.builder();
+    nativeBuilder.Identifier(
+      software.amazon.smithy.dafny.conversion.ToNative.Simple.String(
+        dafnyValue.dtor_Identifier()
+      )
+    );
+    return nativeBuilder.build();
+  }
+
+  public static GetMutationLockOutput GetMutationLockOutput(
+    software.amazon.cryptography.keystore.internaldafny.types.GetMutationLockOutput dafnyValue
+  ) {
+    GetMutationLockOutput.Builder nativeBuilder =
+      GetMutationLockOutput.builder();
+    if (dafnyValue.dtor_mutationLock().is_Some()) {
+      nativeBuilder.mutationLock(
+        ToNative.MutationLock(dafnyValue.dtor_mutationLock().dtor_value())
+      );
+    }
     return nativeBuilder.build();
   }
 
