AwsCryptographicMaterialProviders/runtimes/java/src/main/smithy-generated/software/amazon/cryptography/keystore/model/ClobberMutationLockInput.java
@@ -1,0 +1,88 @@
+// Copyright Amazon.com Inc. or its affiliates. All Rights Reserved.
+// SPDX-License-Identifier: Apache-2.0
+// Do not modify this file. This file is machine generated, and any changes to it will be overwritten.
+package software.amazon.cryptography.keystore.model;
+
+import java.util.Objects;
+
+public class ClobberMutationLockInput {
+
+  /**
+   * Information an in-flight Mutation of a Branch Key.
+   * This ensures:
+   * - only one Mutation affects a Branch Key at a time
+   * - all items of a Branch Key are mutated consistently
+   */
+  private final MutationLock mutationLock;
+
+  protected ClobberMutationLockInput(BuilderImpl builder) {
+    this.mutationLock = builder.mutationLock();
+  }
+
+  /**
+   * @return Information an in-flight Mutation of a Branch Key.
+   * This ensures:
+   * - only one Mutation affects a Branch Key at a time
+   * - all items of a Branch Key are mutated consistently
+   */
+  public MutationLock mutationLock() {
+    return this.mutationLock;
+  }
+
+  public Builder toBuilder() {
+    return new BuilderImpl(this);
+  }
+
+  public static Builder builder() {
+    return new BuilderImpl();
+  }
+
+  public interface Builder {
+    /**
+     * @param mutationLock Information an in-flight Mutation of a Branch Key.
+     * This ensures:
+     * - only one Mutation affects a Branch Key at a time
+     * - all items of a Branch Key are mutated consistently
+     */
+    Builder mutationLock(MutationLock mutationLock);
+
+    /**
+     * @return Information an in-flight Mutation of a Branch Key.
+     * This ensures:
+     * - only one Mutation affects a Branch Key at a time
+     * - all items of a Branch Key are mutated consistently
+     */
+    MutationLock mutationLock();
+
+    ClobberMutationLockInput build();
+  }
+
+  static class BuilderImpl implements Builder {
+
+    protected MutationLock mutationLock;
+
+    protected BuilderImpl() {}
+
+    protected BuilderImpl(ClobberMutationLockInput model) {
+      this.mutationLock = model.mutationLock();
+    }
+
+    public Builder mutationLock(MutationLock mutationLock) {
+      this.mutationLock = mutationLock;
+      return this;
+    }
+
+    public MutationLock mutationLock() {
+      return this.mutationLock;
+    }
+
+    public ClobberMutationLockInput build() {
+      if (Objects.isNull(this.mutationLock())) {
+        throw new IllegalArgumentException(
+          "Missing value for required field `mutationLock`"
+        );
+      }
+      return new ClobberMutationLockInput(this);
+    }
+  }
+}
