AwsCryptographicMaterialProviders/runtimes/java/src/main/smithy-generated/software/amazon/cryptography/keystore/model/GetMutationLockOutput.java
@@ -1,0 +1,69 @@
+// Copyright Amazon.com Inc. or its affiliates. All Rights Reserved.
+// SPDX-License-Identifier: Apache-2.0
+// Do not modify this file. This file is machine generated, and any changes to it will be overwritten.
+package software.amazon.cryptography.keystore.model;
+
+public class GetMutationLockOutput {
+
+  /**
+   * If not present, there is no Mutation Lock.
+   */
+  private final MutationLock mutationLock;
+
+  protected GetMutationLockOutput(BuilderImpl builder) {
+    this.mutationLock = builder.mutationLock();
+  }
+
+  /**
+   * @return If not present, there is no Mutation Lock.
+   */
+  public MutationLock mutationLock() {
+    return this.mutationLock;
+  }
+
+  public Builder toBuilder() {
+    return new BuilderImpl(this);
+  }
+
+  public static Builder builder() {
+    return new BuilderImpl();
+  }
+
+  public interface Builder {
+    /**
+     * @param mutationLock If not present, there is no Mutation Lock.
+     */
+    Builder mutationLock(MutationLock mutationLock);
+
+    /**
+     * @return If not present, there is no Mutation Lock.
+     */
+    MutationLock mutationLock();
+
+    GetMutationLockOutput build();
+  }
+
+  static class BuilderImpl implements Builder {
+
+    protected MutationLock mutationLock;
+
+    protected BuilderImpl() {}
+
+    protected BuilderImpl(GetMutationLockOutput model) {
+      this.mutationLock = model.mutationLock();
+    }
+
+    public Builder mutationLock(MutationLock mutationLock) {
+      this.mutationLock = mutationLock;
+      return this;
+    }
+
+    public MutationLock mutationLock() {
+      return this.mutationLock;
+    }
+
+    public GetMutationLockOutput build() {
+      return new GetMutationLockOutput(this);
+    }
+  }
+}
