AwsCryptographicMaterialProviders/dafny/AwsCryptographyKeyStore/Model/Storage.smithy
@@ -137,7 +137,9 @@ resource KeyStorageInterface {
     GetItemsForInitializeMutation,
     WriteInitializeMutation,
     QueryForVersions,
-    WriteMutatedVersions
+    WriteMutatedVersions,
+    GetMutationLock,
+    ClobberMutationLock
   ]
 }
 
@@ -148,31 +150,44 @@ structure KeyStorageInterfaceReference {}
 operation WriteNewEncryptedBranchKey {
   input: WriteNewEncryptedBranchKeyInput,
   output: WriteNewEncryptedBranchKeyOutput,
+  errors: [
+    KeyStorageException
+    AlreadyExistsConditionFailed
+  ] 
 }
 @documentation("WriteNewEncryptedBranchKeyVersion persists the new active item, decrypt only (version) item of a newly generated Branch Key version.")
 operation WriteNewEncryptedBranchKeyVersion {
   input: WriteNewEncryptedBranchKeyVersionInput,
   output: WriteNewEncryptedBranchKeyVersionOutput,
+  errors: [
+    KeyStorageException
+    AlreadyExistsConditionFailed
+    OldEncConditionFailed
+  ]
 }
 @documentation("Get the ACTIVE branch key for encryption for an existing branch key.")
 operation GetEncryptedActiveBranchKey {
   input: GetEncryptedActiveBranchKeyInput,
   output: GetEncryptedActiveBranchKeyOutput,
+  errors: [ KeyStorageException ]
 }
 @documentation("Get a specific branch key version for an existing branch key.")
 operation GetEncryptedBranchKeyVersion {
   input: GetEncryptedBranchKeyVersionInput,
   output: GetEncryptedBranchKeyVersionOutput,
+  errors: [ KeyStorageException ]
 }
 @documentation("Get the beacon key associated with an existing branch key.")
 operation GetEncryptedBeaconKey {
   input: GetEncryptedBeaconKeyInput,
   output: GetEncryptedBeaconKeyOutput,
+  errors: [ KeyStorageException ]
 }
 @documentation("Gets information about the underlying storage system.")
 operation GetKeyStorageInfo {
   input: GetKeyStorageInfoInput,
-  output: GetKeyStorageInfoOutput,
+  output: GetKeyStorageInfoOutput
+  errors: [ KeyStorageException ]
 }
 
 @documentation(
@@ -195,7 +210,12 @@ Also writes the Mutation Lock.")
 operation WriteInitializeMutation {
   input: WriteInitializeMutationInput
   output: WriteInitializeMutationOutput
-  errors: [KeyStorageException]
+  errors: [
+    KeyStorageException,
+    MutationLockConditionFailed,
+    AlreadyExistsConditionFailed,
+    OldEncConditionFailed
+  ]
 }
 
 @documentation(
@@ -219,7 +239,12 @@ conditioned on:
 operation WriteMutatedVersions {
   input: WriteMutatedVersionsInput
   output: WriteMutatedVersionsOutput
-  errors: [KeyStorageException]
+  errors: [
+    KeyStorageException
+    MutationLockConditionFailed
+    OldEncConditionFailed
+    NoLongerExistsConditionFailed
+  ]
 }
 
 //= aws-encryption-sdk-specification/framework/key-store/key-storage.md#writenewencryptedbranchkey
@@ -470,16 +495,76 @@ structure WriteMutatedVersionsInput {
   @required
   @documentation("A commitment of the Terminal Mutable Properities of the Branch Key.")  
   Terminal: Blob
-  @documentation("If set to True, the Mutation Lock will be deleted. Effectively defaults to false")
+  @documentation("If set to True, the Mutation Lock will be deleted.")
   @required // @default(false) // Smithy-Dafny may not respect defaults.
   CompleteMutation: Boolean
 }
-
-
 structure WriteMutatedVersionsOutput {}
+
+@documentation(
+"Check for Mutation Lock on a Branch Key ID.
+If one exists, returns the Mutation Lock.
+Otherwise, returns nothing.")
+operation GetMutationLock {
+  input: GetMutationLockInput
+  output: GetMutationLockOutput
+  errors: [KeyStorageException]
+}
+structure GetMutationLockInput {
+  @documentation("The Branch Key to check for a Mutation Lock.")
+  @required
+  Identifier: String
+}
+structure GetMutationLockOutput {
+  @documentation("If not present, there is no Mutation Lock.")
+  mutationLock: MutationLock
+}
+
+@documentation("Overwrite an existing Mutation Lock.")
+operation ClobberMutationLock {
+  input: ClobberMutationLockInput
+  output: ClobberMutationLockOutput
+  errors: [
+    KeyStorageException,
+    MutationLockConditionFailed
+  ]
+}
+structure ClobberMutationLockInput {
+  @required
+  mutationLock: MutationLock
+}
+structure ClobberMutationLockOutput {}
 
 @error("client")
 structure KeyStorageException {
   @required
   message: String,
+}
+
+@error("client")
+@documentation("Write to Storage failed due to Mutation Lock condition failure.")
+structure MutationLockConditionFailed {
+  @required
+  message: String
+}
+
+@error("client")
+@documentation("Write to Storage failed. An item already exists for this Branch Key ID & Type.")
+structure AlreadyExistsConditionFailed {
+  @required
+  message: String
+}
+
+@error("client")
+@documentation("Write to Storage failed. Item was deleted since it was read.")
+structure NoLongerExistsConditionFailed {
+  @required
+  message: String
+}
+
+@error("client")
+@documentation("Write to Storage failed; cipher-text attribute of an item was updated since it was read.")
+structure OldEncConditionFailed {
+  @required
+  message: String
 }
